Clap/Lang/All.lean
@@ -1,8 +1,11 @@
 import Clap.Lang.F.F
 import Clap.Lang.F.assert_eq
+import Clap.Lang.F.assert_range
 import Clap.Lang.F.conditionalSwap
 import Clap.Lang.F.dotProduct
 import Clap.Lang.F.guardedEq0
+import Clap.Lang.F.lessThan
+import Clap.Lang.F.num2bits
 import Clap.Lang.FB.assert
 import Clap.Lang.FB.FB
 import Clap.Lang.FB.not
