Clap/Lang/F/assert_range.lean
@@ -1,0 +1,24 @@
+import Clap.Lang.F.F
+import Clap.Lang.F.assert_eq
+import Clap.Lang.F.num2bits
+
+namespace Clap.Edsl.Lang.F
+
+variable {p : ℕ}
+
+/-- Asserts `e` fits in `w` bits, i.e. `e.val < 2^w`. -/
+def assert_range [p.AtLeastTwo] (w : ℕ) (e : F p) : Edsl.CircuitStateM p Unit := do
+  let bits ← num2bits w e
+  assert_eq (bits2num bits) e
+
+namespace assert_range
+
+def spec (p : ℕ) [p.AtLeastTwo] (w : ℕ) : Prop :=
+  matchesUnaryAssertion p (assert_range w) (allocatesN := w)
+    (constraints := fun (v : ZMod p) => v.val < 2^w)
+
+lemma equiv (p : ℕ) [p.AtLeastTwo] (w : ℕ) : spec p w := by sorry
+
+end assert_range
+
+end Clap.Edsl.Lang.F
